\begin{frame}
\frametitle{Properties of Predictive Parsing Grammars}

\begin{enumerate}
\item They are not ambiguous.
\item They are not left recursive (direct or indirect).
\item The FIRST set of each body of a terminal should be disjoint.
\end{enumerate}

\end{frame}


\begin{frame}
\frametitle{Ambiguity}

\begin{block}{Discovering and Removing Ambiguity}
When more than one parse tree can derive the same string of the language, then the grammar is ambiguous.

Proving a grammar ambiguous is an undecidable problem. And there is no algorithm to remove ambiguity from a grammar.

\end{block}

\begin{example}{Ambiguous Grammar}

\texttt{S -> S + S | S - S | 0 | 1 | 2 | 3 | ... | 9}

\vspace{1em}

\texttt{Stmt -> if Expr then Stmt}

\texttt{Stmt -> if Expr then Stmt else Stmt}

\texttt{Stmt -> other}

\end{example}

\end{frame}


\begin{frame}
\frametitle{Eliminating Left Recursion}

\begin{example}{Left Recursion Grammars}
\texttt{E -> E + T}

\texttt{E -> T}

\vspace{1em}

\texttt{A -> Cd}

\texttt{B -> Ce}

\texttt{C -> A | B | f}


\texttt{Stmt -> other}
\end{example}

\begin{block}{Left Recursion can be removed}
Every left-recursive grammar can be converted to a right-recursive grammar.

\vspace{1em}

\texttt{A -> A$\alpha$ | $\beta$}

\vspace{1em}

\texttt{A -> $\beta$A'}

\texttt{A' -> $\alpha$A' | $\epsilon$}

\end{block}

\end{frame}
